cava/arrow-examples/Aes/sbox_canright.v
@@ -115,4 +115,9 @@ Notation "# x" := (nat_to_bitvec_sized 8 x) (at level 99).
 
 Goal combinational_evaluation canright_composed canright_composed_combinational (# 0) = (# 0).
 Proof. vm_compute; auto. Qed.
+
+(* TODO(blaxill): reduced bound for CI time *)
+Goal forall x, x < 10 -> 
+combinational_evaluation canright_composed canright_composed_combinational (#x) = (#x).
+Proof. time (repeat (lia || destruct x); now vm_compute). Qed.
   
